Covalence/Syntax/Basic.lean
@@ -310,6 +310,9 @@ def Tm.b0 (t : Tm) : BSubst | 0 => t | n + 1 => .bv n
 
 @[simp] theorem Tm.get_succ_b0 (t : Tm) (n : ℕ) : t.b0.get (n + 1) = .bv n := rfl
 
+theorem Tm.get_b0 (t : Tm) (n : ℕ) : t.b0.get n = if n = 0 then t else .bv (n - 1)
+  := by cases n <;> rfl
+
 def Tm.bs0 (t : Tm) (s : Tm) : Tm := t.bsubst s.b0
 
 theorem Tm.BSubst.get_liftn (σ : BSubst) (n : ℕ) (i : ℕ)
@@ -337,124 +340,6 @@ theorem Tm.bwk_iter_fv (f : BWk) (n : ℕ) (x : ℕ)
 @[simp]
 theorem Tm.bwk_bwk0_iter_bv (n : ℕ) (i : ℕ)
   : (Tm.bwk BWk.wk0)^[n] (.bv i) = .bv (i + n) := by induction n generalizing i <;> simp +arith [*]
-
-def Tm.FSubst := ℕ → Tm
-
-def Tm.FSubst.get (f : Tm.FSubst) (n : ℕ) : Tm := f n
-
-@[ext] theorem Tm.FSubst.get_ext (f g : Tm.FSubst) (h : ∀ n, f.get n = g.get n) : f = g := funext h
-
-instance Tm.FSubst.instOne : One Tm.FSubst where
-  one := .fv
-
-@[simp] theorem Tm.FSubst.get_one (n : ℕ) : Tm.FSubst.get 1 n = .fv n := rfl
-
-def Tm.FSubst.wkOut (f : BWk) (σ : Tm.FSubst) : Tm.FSubst | n => (σ.get n).bwk f
-
-@[simp] theorem Tm.FSubst.get_wkOut (f : BWk) (σ : Tm.FSubst) (n : ℕ)
-  : (σ.wkOut f).get n = (σ.get n).bwk f := rfl
-
-theorem Tm.FSubst.wkOut_wkOut (f g : BWk) (σ : Tm.FSubst) :
-  (σ.wkOut f).wkOut g = σ.wkOut (g * f) := by ext n; simp [bwk_bwk]
-
-def Tm.FSubst.lift (f : Tm.FSubst) : Tm.FSubst := f.wkOut .wk0
-
-prefix:75 "↑f " => Tm.FSubst.lift
-
-@[simp] theorem Tm.FSubst.get_lift (f : Tm.FSubst) (n : ℕ) : (↑f f).get n = ↑0 (f.get n) := rfl
-
-@[simp] theorem Tm.FSubst.lift_one : ↑f 1 = 1 := by ext n; cases n <;> rfl
-
-theorem Tm.FSubst.lift_wkOut_wk0 (f : BWk) (σ : Tm.FSubst) :
-  ↑f (σ.wkOut f) = σ.wkOut (.wk0 * f) := by rw [lift, wkOut_wkOut]
-
-theorem Tm.FSubst.lift_wkOut_lift (f : BWk) (σ : Tm.FSubst) :
-  (↑f σ).wkOut (↑b f) = ↑f (σ.wkOut f) := by ext n; simp [bwk_bwk, BWk.lift_mul_wk0]
-
-theorem Tm.FSubst.lift_wkOut (f : BWk) (σ : Tm.FSubst) :
-  ↑f (σ.wkOut f) = (↑f σ).wkOut (↑b f) := by rw [lift_wkOut_lift]
-
-@[simp]
-def Tm.fsubst (σ : FSubst) : Tm → Tm
-  | .fv x => σ.get x
-  | .bv i => .bv i
-  | .univ ℓ => .univ ℓ
-  | .unit ℓ => .unit ℓ
-  | .nil ℓ => .nil ℓ
-  | .empty ℓ => .empty ℓ
-  | .eqn A a b => .eqn (A.fsubst σ) (a.fsubst σ) (b.fsubst σ)
-  | .pi ℓ A B => .pi ℓ (A.fsubst σ) (B.fsubst (↑f σ))
-  | .abs ℓ A B b => .abs ℓ (A.fsubst σ) (B.fsubst (↑f σ)) (b.fsubst (↑f σ))
-  | .app ℓ A B f a => .app ℓ (A.fsubst σ) (B.fsubst (↑f σ)) (f.fsubst σ) (a.fsubst σ)
-  | .sigma ℓ A B => .sigma ℓ (A.fsubst σ) (B.fsubst (↑f σ))
-  | .pair ℓ A B a b => .pair ℓ (A.fsubst σ) (B.fsubst (↑f σ)) (a.fsubst σ) (b.fsubst σ)
-  | .fst ℓ A B a => .fst ℓ (A.fsubst σ) (B.fsubst (↑f σ)) (a.fsubst σ)
-  | .snd ℓ A B a => .snd ℓ (A.fsubst σ) (B.fsubst (↑f σ)) (a.fsubst σ)
-  | .dite φ A a b => .dite (φ.fsubst σ) (A.fsubst σ) (a.fsubst σ) (b.fsubst σ)
-  | .trunc A => .trunc (A.fsubst σ)
-  | .choose A φ => .choose (A.fsubst σ) (φ.fsubst (↑f σ))
-  | .nats => .nats
-  | .zero => .zero
-  | .succ => .succ
-  | .natrec C n z s => .natrec (C.fsubst (↑f σ)) (n.fsubst σ) (z.fsubst σ) (s.fsubst (↑f σ))
-  | .let₁ A a b => .let₁ (A.fsubst σ) (a.fsubst σ) (b.fsubst (↑f σ))
-  | .invalid => .invalid
-
-@[simp]
-theorem Tm.fsubst_one (t : Tm) : t.fsubst 1 = t := by induction t <;> simp [*]
-
-instance Tm.FSubst.instMul : Mul Tm.FSubst where
-  mul f g := fun n => (g.get n).fsubst f
-
-@[simp]
-theorem Tm.FSubst.get_mul (f g : Tm.FSubst) (n : ℕ) : (f * g).get n = (g.get n).fsubst f := rfl
-
-theorem Tm.bwk_fsubst_wkOut (f : BWk) (σ : Tm.FSubst) (t : Tm) :
-  (t.bwk f).fsubst (σ.wkOut f) = (t.fsubst σ).bwk f := by
-  induction t generalizing f σ <;> simp [FSubst.lift_wkOut, *]
-
-theorem Tm.bwk_fsubst (t : Tm) (f : BWk) (σ : Tm.FSubst) :
-   (t.fsubst σ).bwk f = (t.bwk f).fsubst (σ.wkOut f) := by rw [bwk_fsubst_wkOut]
-
-theorem Tm.wk0_fsubst_lift (σ : Tm.FSubst) (t : Tm) : (↑0 t).fsubst (↑f σ) = ↑0 (t.fsubst σ)
-  := bwk_fsubst_wkOut .wk0 σ t
-
-theorem Tm.FSubst.lift_mul (f g : Tm.FSubst) : ↑f (f * g) = ↑f f * ↑f g
-  := by ext n; simp [Tm.wk0_fsubst_lift]
-
-theorem Tm.fsubst_mul (t : Tm) (f g : FSubst) : t.fsubst (f * g) = (t.fsubst g).fsubst f := by
-  induction t generalizing f g <;> simp [FSubst.lift_mul, *]
-
-instance Tm.FSubst.instMonoid : Monoid Tm.FSubst where
-  mul_assoc f g h := by ext n; simp [fsubst_mul]
-  one_mul f := by ext n; simp
-  mul_one f := by ext n; simp
-
-def Tm.FSubst.bsubstOut (f : BSubst) (σ : Tm.FSubst) : FSubst | x => (σ.get x).bsubst f
-
-@[simp]
-theorem Tm.FSubst.get_bsubstOut (f : BSubst) (σ : Tm.FSubst) (x : ℕ) :
-  (σ.bsubstOut f).get x = (σ.get x).bsubst f := rfl
-
--- theorem Tm.FSubst.lift_bsubstOut_wk0 (f : BSubst) (σ : Tm.FSubst) :
---   ↑f (σ.bsubstOut f) = σ.bsubstOut (f.wkOut .wk0) := by sorry
-
-theorem Tm.FSubst.lift_bsubstOut_lift (f : BSubst) (σ : Tm.FSubst) :
-  (↑f σ).bsubstOut (↑s f) = ↑f (σ.bsubstOut f) := by ext n; simp [bsubst_lift_wk0]
-
-theorem Tm.FSubst.lift_bsubstOut (f : BSubst) (σ : Tm.FSubst) :
-  ↑f (σ.bsubstOut f) = (↑f σ).bsubstOut (↑s f) := by rw [lift_bsubstOut_lift]
-
--- theorem Tm.bsubst_fsubst (t : Tm) (f : BSubst) (σ : Tm.FSubst) :
---   (t.fsubst σ).bsubst f = (t.bsubst f).fsubst (σ.bsubstOut f) := by
---   induction t generalizing σ f <;> simp [*]
---   sorry
-
-def Tm.BSubst.fsubstOut (σ : Tm.FSubst) (f : BSubst) : BSubst | i => (f.get i).fsubst σ
-
-@[simp]
-theorem Tm.BSubst.get_fsubstOut (σ : Tm.FSubst) (f : BSubst) (i : ℕ) :
-  (f.fsubstOut σ).get i = (f.get i).fsubst σ := rfl
 
 @[simp]
 theorem Tm.fvs_bwk (t : Tm) (f : BWk) : (t.bwk f).fvs = t.fvs
@@ -844,3 +729,12 @@ theorem Tm.bs0_lc_of (t : Tm) (s : Tm) (ht : t.bvi ≤ 1) (hs : s.bvi = 0) : (t.
 --       bvs, Set.mem_empty_iff_false, Set.mem_union, mem_liftBvSet_iff, bsubst, bvi
 --     ] at * <;>
 --     sorry
+
+theorem Tm.lc_bvs_of_bwk_lc (t : Tm) (f : BWk) (h : (t.bwk f).bvs = ∅) : t.bvs = ∅ := by
+  rw [Tm.bvs_bwk, Set.eq_empty_iff_forall_notMem] at h
+  simp only [Set.mem_setOf_eq, not_exists, not_and, forall_apply_eq_imp_iff₂, imp_false] at h
+  rw [Set.eq_empty_iff_forall_notMem]
+  exact h
+
+theorem Tm.lc_of_bwk_lc (t : Tm) (f : BWk) (h : (t.bwk f).bvi = 0) : t.bvi = 0 :=
+  by simp only [<-Tm.bvs_emp_iff] at *; exact lc_bvs_of_bwk_lc _ _ h
