Covalence/Syntax.lean
@@ -1,2 +1,3 @@
 import Covalence.Syntax.Basic
 import Covalence.Syntax.MSubst
+import Covalence.Syntax.FSubst
